LeanFunge/Theory/Completeness.lean
@@ -3,6 +3,10 @@ Copyright (c) 2026 Bangyen Pham. All rights reserved.
 Released under Apache 2.0 license as described in the file LICENSE.
 Authors: Bangyen Pham
 -/
+import LeanFunge.Theory.Completeness.Linear
+import LeanFunge.Theory.Completeness.LinearMain
+import LeanFunge.Theory.Completeness.LinearRow
+import LeanFunge.Theory.Completeness.LinearSimulation
 import LeanFunge.Theory.Completeness.PairEncoding
 import LeanFunge.Theory.Completeness.Routing
 import LeanFunge.Theory.Completeness.Simulation
