Tests/Completeness/Linear.lean
@@ -1,0 +1,72 @@
+/-
+Copyright (c) 2026 Bangyen Pham. All rights reserved.
+Released under Apache 2.0 license as described in the file LICENSE.
+Authors: Bangyen Pham
+-/
+import LeanFunge.Theory.Completeness.LinearMain
+
+/-!
+# Branch-Free Simulation Tests
+-/
+
+namespace LeanFunge.Tests
+
+open LeanFunge.Completeness
+
+example (c : Fin 2) : (linearCells (.inc c)).length = 2 :=
+  linearCells_length_inc c
+
+example (prog : CMProgram) (j : ℕ)
+    (hinc : ∀ i, i < j → prog.getD i .halt = .inc 0 ∨ prog.getD i .halt = .inc 1) :
+    (linearRowAux prog).drop (2 * j) = linearRowAux (prog.drop j) :=
+  linearRowAux_drop prog j hinc
+
+example (prog : CMProgram) (j : ℕ)
+    (hinc : ∀ i, i < j → prog.getD i .halt = .inc 0 ∨ prog.getD i .halt = .inc 1)
+    (hjinc : prog.getD j .halt = .inc 0 ∨ prog.getD j .halt = .inc 1) :
+    (linearRow prog).getD (1 + 2 * j) ' ' = (linearCells (prog.getD j .halt)).getD 0 ' ' :=
+  linearRow_get_first prog j hinc hjinc
+
+example (prog : CMProgram) (j : ℕ)
+    (hinc : ∀ i, i < j → prog.getD i .halt = .inc 0 ∨ prog.getD i .halt = .inc 1) :
+    1 + 2 * j < (linearRow prog).length :=
+  linearRow_length prog j hinc
+
+example (prog : CMProgram) (j : ℕ) (c : Fin 2) (s : CMState)
+    (h : prog.getD j .halt = .inc c) :
+    foldIncs prog (j + 1) s = CMInstr.incCounter c (foldIncs prog j s) :=
+  foldIncs_succ_inc prog j c s h
+
+example (prog : CMProgram) (c1 c2 : ℕ) {j : ℕ}
+    (h : prog.getD j .halt = .inc 0) :
+    (Int.ofNat (encode (foldIncs prog j (CMInstr.startCM c1 c2)).c1
+                       (foldIncs prog j (CMInstr.startCM c1 c2)).c2)) * 2
+      = Int.ofNat (encode (foldIncs prog (j + 1) (CMInstr.startCM c1 c2)).c1
+                          (foldIncs prog (j + 1) (CMInstr.startCM c1 c2)).c2) :=
+  enc_update_inc_zero prog c1 c2 h
+
+example (prog : CMProgram) (c1 c2 : ℕ) (j : ℕ)
+    (hinc : ∀ i, i < j → prog.getD i .halt = .inc 0 ∨ prog.getD i .halt = .inc 1)
+    (hw : 1 + 2 * j < (linearRow prog).length) :
+    run (1 + 2 * j) (linearStart prog c1 c2) =
+      some { linearStart prog c1 c2 with
+        stack := [Int.ofNat (encode (foldIncs prog j (CMInstr.startCM c1 c2)).c1
+                                     (foldIncs prog j (CMInstr.startCM c1 c2)).c2)],
+        pc := (1 + 2 * j, 0) } :=
+  linear_prefix prog c1 c2 j hinc hw
+
+example (prog : CMProgram) (c1 c2 : ℕ) (hpos : 0 < prog.length)
+    (hinc : ∀ i, i + 1 < prog.length → prog.getD i .halt = .inc 0 ∨ prog.getD i .halt = .inc 1) :
+    (run (1 + 2 * (prog.length - 1)) (linearStart prog c1 c2)).map (fun s => s.stack)
+      = some [Int.ofNat (encode (foldIncs prog (prog.length - 1) (CMInstr.startCM c1 c2)).c1
+                                 (foldIncs prog (prog.length - 1) (CMInstr.startCM c1 c2)).c2)] :=
+  linear_stack prog c1 c2 hpos hinc
+
+example (prog : CMProgram) (c1 c2 : ℕ) (hpos : 0 < prog.length)
+    (hinc : ∀ i, i + 1 < prog.length → prog.getD i .halt = .inc 0 ∨ prog.getD i .halt = .inc 1) :
+    (run (1 + 2 * (prog.length - 1)) (linearStart prog c1 c2)).map (fun s => s.stack)
+      = (CMInstr.run prog (prog.length - 1) (CMInstr.startCM c1 c2)).map
+          (fun s => [Int.ofNat (encode s.c1 s.c2)]) :=
+  linear_simulation prog c1 c2 hpos hinc
+
+end LeanFunge.Tests
